Add comments for message formats + some fixes

fstar/treedem/MLS.TreeDEM.NetworkTypes.fst
@@ -7,11 +7,26 @@ open MLS.TreeKEM.NetworkTypes
 
 (*** PSKs ***)
 
+/// enum {
+///   reserved(0),
+///   external(1),
+///   resumption(2),
+///   (255)
+/// } PSKType;
+
 type psk_type_nt =
   | [@@@ with_num_tag 1 1] PSKT_external: psk_type_nt
   | [@@@ with_num_tag 1 2] PSKT_resumption: psk_type_nt
 
 %splice [ps_psk_type_nt] (gen_parser (`psk_type_nt))
+
+/// enum {
+///   reserved(0),
+///   application(1),
+///   reinit(2),
+///   branch(3),
+///   (255)
+/// } ResumptionPSKUsage;
 
 type resumption_psk_usage_nt =
   | [@@@ with_num_tag 1 1] RPSKU_application: resumption_psk_usage_nt
@@ -20,11 +35,31 @@ type resumption_psk_usage_nt =
 
 %splice [ps_resumption_psk_usage_nt] (gen_parser (`resumption_psk_usage_nt))
 
+/// struct {
+///   PSKType psktype;
+///   select (PreSharedKeyID.psktype) {
+///     case external:
+///       opaque psk_id<V>;
+///
+///     case resumption:
+///       ResumptionPSKUsage usage;
+///       opaque psk_group_id<V>;
+///       uint64 psk_epoch;
+///   };
+///   opaque psk_nonce<V>;
+/// } PreSharedKeyID;
+
 type pre_shared_key_id_nt (bytes:Type0) {|bytes_like bytes|} =
   | [@@@ with_tag PSKT_external] PSKI_external: psk_id:mls_bytes bytes -> psk_nonce:mls_bytes bytes -> pre_shared_key_id_nt bytes
   | [@@@ with_tag PSKT_resumption] PSKI_resumption: usage: resumption_psk_usage_nt -> psk_group_id:mls_bytes bytes -> psk_epoch:nat_lbytes 8 -> psk_nonce:mls_bytes bytes -> pre_shared_key_id_nt bytes
 
 %splice [ps_pre_shared_key_id_nt] (gen_parser (`pre_shared_key_id_nt))
+
+/// struct {
+///     PreSharedKeyID id;
+///     uint16 index;
+///     uint16 count;
+/// } PSKLabel;
 
 type psk_label_nt (bytes:Type0) {|bytes_like bytes|} = {
   id: pre_shared_key_id_nt bytes;
@@ -38,11 +73,19 @@ instance parseable_serializeable_psk_label_nt (bytes:Type0) {|bytes_like bytes|}
 
 (*** Proposals ***)
 
+/// struct {
+///     KeyPackage key_package;
+/// } Add;
+
 type add_nt (bytes:Type0) {|bytes_like bytes|} = {
   key_package: key_package_nt bytes tkt;
 }
 
 %splice [ps_add_nt] (gen_parser (`add_nt))
+
+/// struct {
+///     LeafNode leaf_node;
+/// } Update;
 
 type update_nt (bytes:Type0) {|bytes_like bytes|} = {
   leaf_node: leaf_node_nt bytes tkt;
@@ -50,17 +93,32 @@ type update_nt (bytes:Type0) {|bytes_like bytes|} = {
 
 %splice [ps_update_nt] (gen_parser (`update_nt))
 
+/// struct {
+///     uint32 removed;
+/// } Remove;
+
 type remove_nt (bytes:Type0) {|bytes_like bytes|} = {
   removed: nat_lbytes 4;
 }
 
 %splice [ps_remove_nt] (gen_parser (`remove_nt))
 
+/// struct {
+///     PreSharedKeyID psk;
+/// } PreSharedKey;
+
 type pre_shared_key_nt (bytes:Type0) {|bytes_like bytes|} = {
   psk: pre_shared_key_id_nt bytes;
 }
 
 %splice [ps_pre_shared_key_nt] (gen_parser (`pre_shared_key_nt))
+
+/// struct {
+///     opaque group_id<V>;
+///     ProtocolVersion version;
+///     CipherSuite cipher_suite;
+///     Extension extensions<V>;
+/// } ReInit;
 
 type reinit_nt (bytes:Type0) {|bytes_like bytes|} = {
   group_id: mls_bytes bytes;
@@ -71,11 +129,19 @@ type reinit_nt (bytes:Type0) {|bytes_like bytes|} = {
 
 %splice [ps_reinit_nt] (gen_parser (`reinit_nt))
 
+/// struct {
+///   opaque kem_output<V>;
+/// } ExternalInit;
+
 type external_init_nt (bytes:Type0) {|bytes_like bytes|} = {
   kem_output: mls_bytes bytes
 }
 
 %splice [ps_external_init_nt] (gen_parser (`external_init_nt))
+
+/// struct {
+///   Extension extensions<V>;
+/// } GroupContextExtensions;
 
 type group_context_extensions_nt (bytes:Type0) {|bytes_like bytes|} = {
   extensions: mls_list bytes ps_extension_nt;
@@ -85,6 +151,11 @@ type group_context_extensions_nt (bytes:Type0) {|bytes_like bytes|} = {
 
 (*** Refs ***)
 
+/// opaque HashReference<V>;
+///
+/// HashReference KeyPackageRef;
+/// HashReference ProposalRef;
+
 type key_package_ref_nt (bytes:Type0) {|bytes_like bytes|} = mls_bytes bytes
 %splice [ps_key_package_ref_nt] (gen_parser (`key_package_ref_nt))
 
@@ -92,6 +163,9 @@ type proposal_ref_nt (bytes:Type0) {|bytes_like bytes|} = mls_bytes bytes
 %splice [ps_proposal_ref_nt] (gen_parser (`proposal_ref_nt))
 
 (*** Message framing ***)
+
+/// // See IANA registry for registered values
+/// uint16 ProposalType;
 
 type proposal_nt (bytes:Type0) {|bytes_like bytes|} =
   | [@@@ with_tag PT_add] P_add: add_nt bytes -> proposal_nt bytes
@@ -104,11 +178,31 @@ type proposal_nt (bytes:Type0) {|bytes_like bytes|} =
 
 %splice [ps_proposal_nt] (gen_parser (`proposal_nt))
 
+/// enum {
+///   reserved(0),
+///   proposal(1),
+///   reference(2),
+///   (255)
+/// } ProposalOrRefType;
+///
+/// struct {
+///   ProposalOrRefType type;
+///   select (ProposalOrRef.type) {
+///     case proposal:  Proposal proposal;
+///     case reference: ProposalRef reference;
+///   };
+/// } ProposalOrRef;
+
 type proposal_or_ref_nt (bytes:Type0) {|bytes_like bytes|} =
   | [@@@ with_num_tag 1 1] POR_proposal: proposal_nt bytes -> proposal_or_ref_nt bytes
   | [@@@ with_num_tag 1 2] POR_reference: proposal_ref_nt bytes -> proposal_or_ref_nt bytes
 
 %splice [ps_proposal_or_ref_nt] (gen_parser (`proposal_or_ref_nt))
+
+/// struct {
+///     ProposalOrRef proposals<V>;
+///     optional<UpdatePath> path;
+/// } Commit;
 
 type commit_nt (bytes:Type0) {|bytes_like bytes|} = {
   proposals: mls_list bytes ps_proposal_or_ref_nt;
@@ -118,6 +212,15 @@ type commit_nt (bytes:Type0) {|bytes_like bytes|} = {
 
 %splice [ps_commit_nt] (gen_parser (`commit_nt))
 
+/// enum {
+///     reserved(0),
+///     member(1),
+///     external(2),
+///     new_member_proposal(3),
+///     new_member_commit(4),
+///     (255)
+/// } SenderType;
+
 type sender_type_nt =
   | [@@@ with_num_tag 1 1] ST_member: sender_type_nt
   | [@@@ with_num_tag 1 2] ST_external: sender_type_nt
@@ -126,6 +229,19 @@ type sender_type_nt =
 
 %splice [ps_sender_type_nt] (gen_parser (`sender_type_nt))
 
+/// struct {
+///     SenderType sender_type;
+///     select (Sender.sender_type) {
+///         case member:
+///             uint32 leaf_index;
+///         case external:
+///             uint32 sender_index;
+///         case new_member_commit:
+///         case new_member_proposal:
+///             struct{};
+///     };
+/// } Sender;
+
 type sender_nt (bytes:Type0) {|bytes_like bytes|} =
   | [@@@ with_tag ST_member] S_member: leaf_index:nat_lbytes 4 -> sender_nt bytes
   | [@@@ with_tag ST_external] S_external: sender_index:nat_lbytes 4 -> sender_nt bytes
@@ -133,6 +249,9 @@ type sender_nt (bytes:Type0) {|bytes_like bytes|} =
   | [@@@ with_tag ST_new_member_commit] S_new_member_commit: sender_nt bytes
 
 %splice [ps_sender_nt] (gen_parser (`sender_nt))
+
+/// // See IANA registry for registered values
+/// uint16 WireFormat;
 
 type wire_format_nt =
   | [@@@ with_num_tag 2 0] WF_reserved: wire_format_nt
@@ -145,8 +264,18 @@ type wire_format_nt =
 
 %splice [ps_wire_format_nt] (gen_parser (`wire_format_nt))
 
+/// opaque MAC<V>;
+
 type mac_nt (bytes:Type0) {|bytes_like bytes|} = mls_bytes bytes
 %splice [ps_mac_nt] (gen_parser (`mac_nt))
+
+/// enum {
+///     reserved(0),
+///     application(1),
+///     proposal(2),
+///     commit(3),
+///     (255)
+/// } ContentType;
 
 type content_type_nt =
   | [@@@ with_num_tag 1 1] CT_application: content_type_nt
@@ -154,6 +283,23 @@ type content_type_nt =
   | [@@@ with_num_tag 1 3] CT_commit: content_type_nt
 
 %splice [ps_content_type_nt] (gen_parser (`content_type_nt))
+
+/// struct {
+///     opaque group_id<V>;
+///     uint64 epoch;
+///     Sender sender;
+///     opaque authenticated_data<V>;
+///
+///     ContentType content_type;
+///     select (FramedContent.content_type) {
+///         case application:
+///           opaque application_data<V>;
+///         case proposal:
+///           Proposal proposal;
+///         case commit:
+///           Commit commit;
+///     };
+/// } FramedContent;
 
 val mls_untagged_content_nt: bytes:Type0 -> {|bytes_like bytes|} -> content_type_nt -> Type0
 let mls_untagged_content_nt bytes #bl content_type =
@@ -181,6 +327,20 @@ type framed_content_nt (bytes:Type0) {|bytes_like bytes|} = {
 
 %splice [ps_framed_content_nt] (gen_parser (`framed_content_nt))
 
+/// struct {
+///     ProtocolVersion version = mls10;
+///     WireFormat wire_format;
+///     FramedContent content;
+///     select (FramedContentTBS.content.sender.sender_type) {
+///         case member:
+///         case new_member_commit:
+///             GroupContext context;
+///         case external:
+///         case new_member_proposal:
+///             struct{};
+///     };
+/// } FramedContentTBS;
+
 let framed_content_tbs_group_context_nt (bytes:Type0) {|bytes_like bytes|} (s:sender_nt bytes) =
   match s with
   | S_member _
@@ -191,6 +351,7 @@ let framed_content_tbs_group_context_nt (bytes:Type0) {|bytes_like bytes|} (s:se
 %splice [ps_framed_content_tbs_group_context_nt] (gen_parser_prefix (`framed_content_tbs_group_context_nt))
 
 type framed_content_tbs_nt (bytes:Type0) {|bytes_like bytes|} = {
+  version: protocol_version_nt;
   wire_format: wire_format_nt;
   content: framed_content_nt bytes;
   group_context: framed_content_tbs_group_context_nt bytes (content.sender);
@@ -199,6 +360,22 @@ type framed_content_tbs_nt (bytes:Type0) {|bytes_like bytes|} = {
 %splice [ps_framed_content_tbs_nt] (gen_parser (`framed_content_tbs_nt))
 
 instance parseable_serializeable_framed_content_tbs_nt (bytes:Type0) {|bytes_like bytes|}: parseable_serializeable bytes (framed_content_tbs_nt bytes) = mk_parseable_serializeable ps_framed_content_tbs_nt
+
+/// struct {
+///     /* SignWithLabel(., "FramedContentTBS", FramedContentTBS) */
+///     opaque signature<V>;
+///     select (FramedContent.content_type) {
+///         case commit:
+///             /*
+///               MAC(confirmation_key,
+///                   GroupContext.confirmed_transcript_hash)
+///             */
+///             MAC confirmation_tag;
+///         case application:
+///         case proposal:
+///             struct{};
+///     };
+/// } FramedContentAuthData;
 
 val confirmation_tag_nt: bytes:Type0 -> {|bytes_like bytes|} -> content_type_nt -> Type0
 let confirmation_tag_nt bytes #bl content =
@@ -215,6 +392,12 @@ type framed_content_auth_data_nt (bytes:Type0) {|bl:bytes_like bytes|} (content_
 
 %splice [ps_framed_content_auth_data_nt] (gen_parser (`framed_content_auth_data_nt))
 
+/// struct {
+///     WireFormat wire_format;
+///     FramedContent content;
+///     FramedContentAuthData auth;
+/// } AuthenticatedContent;
+
 type authenticated_content_nt (bytes:Type0) {|bytes_like bytes|} = {
   wire_format: wire_format_nt;
   content: framed_content_nt bytes;
@@ -222,6 +405,11 @@ type authenticated_content_nt (bytes:Type0) {|bytes_like bytes|} = {
 }
 
 %splice [ps_authenticated_content_nt] (gen_parser (`authenticated_content_nt))
+
+/// struct {
+///   FramedContentTBS content_tbs;
+///   FramedContentAuthData auth;
+/// } AuthenticatedContentTBM;
 
 type authenticated_content_tbm_nt (bytes:Type0) {|bytes_like bytes|} = {
   content_tbs: framed_content_tbs_nt bytes;
@@ -231,6 +419,19 @@ type authenticated_content_tbm_nt (bytes:Type0) {|bytes_like bytes|} = {
 %splice [ps_authenticated_content_tbm_nt] (gen_parser (`authenticated_content_tbm_nt))
 
 instance parseable_serializeable_authenticated_content_tbm_nt (bytes:Type0) {|bytes_like bytes|}: parseable_serializeable bytes (authenticated_content_tbm_nt bytes) = mk_parseable_serializeable ps_authenticated_content_tbm_nt
+
+/// struct {
+///     FramedContent content;
+///     FramedContentAuthData auth;
+///     select (PublicMessage.content.sender.sender_type) {
+///         case member:
+///             MAC membership_tag;
+///         case external:
+///         case new_member_commit:
+///         case new_member_proposal:
+///             struct{};
+///     };
+/// } PublicMessage;
 
 let membership_tag_nt (bytes:Type0) {|bytes_like bytes|} (s:sender_nt bytes) =
   match s with
@@ -247,6 +448,15 @@ type public_message_nt (bytes:Type0) {|bytes_like bytes|} = {
 
 %splice [ps_public_message_nt] (gen_parser (`public_message_nt))
 
+/// struct {
+///     opaque group_id<V>;
+///     uint64 epoch;
+///     ContentType content_type;
+///     opaque authenticated_data<V>;
+///     opaque encrypted_sender_data<V>;
+///     opaque ciphertext<V>;
+/// } PrivateMessage;
+
 type private_message_nt (bytes:Type0) {|bytes_like bytes|} = {
   group_id: mls_bytes bytes;
   epoch: nat_lbytes 8;
@@ -258,33 +468,56 @@ type private_message_nt (bytes:Type0) {|bytes_like bytes|} = {
 
 %splice [ps_private_message_nt] (gen_parser (`private_message_nt))
 
-type private_content_tbe_data_nt (bytes:Type0) {|bytes_like bytes|} (content_type: content_type_nt) = {
+/// struct {
+///     select (PrivateMessage.content_type) {
+///         case application:
+///           opaque application_data<V>;
+///
+///         case proposal:
+///           Proposal proposal;
+///
+///         case commit:
+///           Commit commit;
+///     };
+///
+///     FramedContentAuthData auth;
+///     opaque padding[length_of_padding];
+/// } PrivateMessageContent;
+
+type private_message_content_data_nt (bytes:Type0) {|bytes_like bytes|} (content_type: content_type_nt) = {
   content: mls_untagged_content_nt bytes content_type;
   auth: framed_content_auth_data_nt bytes content_type;
 }
 
-%splice [ps_private_content_tbe_data_nt] (gen_parser (`private_content_tbe_data_nt))
+%splice [ps_private_message_content_data_nt] (gen_parser (`private_message_content_data_nt))
 
 let is_nat_zero (n:nat_lbytes 1) = n = 0
 let zero_byte = refined (nat_lbytes 1) is_nat_zero
 let ps_zero_byte (#bytes:Type0) {|bytes_like bytes|} = refine #bytes (ps_nat_lbytes 1) is_nat_zero
 
-type private_content_tbe_nt (bytes:Type0) {|bytes_like bytes|} (content_type: content_type_nt) = {
-  data: private_content_tbe_data_nt bytes content_type;
+type private_message_content_nt (bytes:Type0) {|bytes_like bytes|} (content_type: content_type_nt) = {
+  data: private_message_content_data_nt bytes content_type;
   padding: list zero_byte;
 }
 
-val pse_private_content_tbe_nt: #bytes:Type0 -> {|bytes_like bytes|} -> content_type:content_type_nt -> parser_serializer_whole bytes (private_content_tbe_nt bytes content_type)
-let pse_private_content_tbe_nt #bytes #bl content_type =
+val pse_private_message_content_nt: #bytes:Type0 -> {|bytes_like bytes|} -> content_type:content_type_nt -> parser_serializer_whole bytes (private_message_content_nt bytes content_type)
+let pse_private_message_content_nt #bytes #bl content_type =
   let iso = mk_isomorphism_between
     (fun (|data, padding|) -> {data; padding})
     (fun {data; padding} -> (|data, padding|))
   in
   isomorphism_whole
-    (bind_whole (ps_private_content_tbe_data_nt content_type) (fun _ -> ps_whole_list ps_zero_byte))
+    (bind_whole (ps_private_message_content_data_nt content_type) (fun _ -> ps_whole_list ps_zero_byte))
     iso
 
-instance parseable_serializeable_private_content_tbe_nt (bytes:Type0) {|bytes_like bytes|} (content_type:content_type_nt): parseable_serializeable bytes (private_content_tbe_nt bytes content_type) = mk_parseable_serializeable_from_whole (pse_private_content_tbe_nt content_type)
+instance parseable_serializeable_private_message_content_nt (bytes:Type0) {|bytes_like bytes|} (content_type:content_type_nt): parseable_serializeable bytes (private_message_content_nt bytes content_type) = mk_parseable_serializeable_from_whole (pse_private_message_content_nt content_type)
+
+/// struct {
+///     opaque group_id<V>;
+///     uint64 epoch;
+///     ContentType content_type;
+///     opaque authenticated_data<V>;
+/// } PrivateContentAAD;
 
 type private_content_aad_nt (bytes:Type0) {|bytes_like bytes|} = {
   group_id: mls_bytes bytes;
@@ -297,6 +530,12 @@ type private_content_aad_nt (bytes:Type0) {|bytes_like bytes|} = {
 
 instance parseable_serializeable_private_content_aad_nt (bytes:Type0) {|bytes_like bytes|}: parseable_serializeable bytes (private_content_aad_nt bytes) = mk_parseable_serializeable ps_private_content_aad_nt
 
+/// struct {
+///     uint32 leaf_index;
+///     uint32 generation;
+///     opaque reuse_guard[4];
+/// } SenderData;
+
 type sender_data_nt (bytes:Type0) {|bytes_like bytes|} = {
   leaf_index: nat_lbytes 4;
   generation: nat_lbytes 4;
@@ -306,6 +545,12 @@ type sender_data_nt (bytes:Type0) {|bytes_like bytes|} = {
 %splice [ps_sender_data_nt] (gen_parser (`sender_data_nt))
 
 instance parseable_serializeable_sender_data_nt (bytes:Type0) {|bytes_like bytes|}: parseable_serializeable bytes (sender_data_nt bytes) = mk_parseable_serializeable ps_sender_data_nt
+
+/// struct {
+///     opaque group_id<V>;
+///     uint64 epoch;
+///     ContentType content_type;
+/// } SenderDataAAD;
 
 type sender_data_aad_nt (bytes:Type0) {|bytes_like bytes|} = {
   group_id: mls_bytes bytes;
@@ -317,6 +562,12 @@ type sender_data_aad_nt (bytes:Type0) {|bytes_like bytes|} = {
 
 instance parseable_serializeable_sender_data_aad_nt (bytes:Type0) {|bytes_like bytes|}: parseable_serializeable bytes (sender_data_aad_nt bytes) = mk_parseable_serializeable ps_sender_data_aad_nt
 
+/// struct {
+///     WireFormat wire_format;
+///     FramedContent content; /* with content_type == commit */
+///     opaque signature<V>;
+/// } ConfirmedTranscriptHashInput;
+
 type confirmed_transcript_hash_input_nt (bytes:Type0) {|bytes_like bytes|} = {
   wire_format: wire_format_nt;
   content: framed_content_nt bytes;
@@ -327,6 +578,10 @@ type confirmed_transcript_hash_input_nt (bytes:Type0) {|bytes_like bytes|} = {
 
 instance parseable_serializeable_confirmed_transcript_hash_input_nt (bytes:Type0) {|bytes_like bytes|}: parseable_serializeable bytes (confirmed_transcript_hash_input_nt bytes) = mk_parseable_serializeable ps_confirmed_transcript_hash_input_nt
 
+/// struct {
+///     MAC confirmation_tag;
+/// } InterimTranscriptHashInput;
+
 type interim_transcript_hash_input_nt (bytes:Type0) {|bytes_like bytes|} = {
   confirmation_tag: mac_nt bytes;
 }
@@ -334,6 +589,13 @@ type interim_transcript_hash_input_nt (bytes:Type0) {|bytes_like bytes|} = {
 %splice [ps_interim_transcript_hash_input_nt] (gen_parser (`interim_transcript_hash_input_nt))
 
 instance parseable_serializeable_interim_transcript_hash_input_nt (bytes:Type0) {|bytes_like bytes|}: parseable_serializeable bytes (interim_transcript_hash_input_nt bytes) = mk_parseable_serializeable ps_interim_transcript_hash_input_nt
+
+/// struct {
+///     GroupContext group_context;
+///     Extension extensions<V>;
+///     MAC confirmation_tag;
+///     uint32 signer;
+/// } GroupInfoTBS;
 
 type group_info_tbs_nt (bytes:Type0) {|bytes_like bytes|} = {
   group_context: group_context_nt bytes;
@@ -346,6 +608,15 @@ type group_info_tbs_nt (bytes:Type0) {|bytes_like bytes|} = {
 
 instance parseable_serializeable_group_info_tbs_nt (bytes:Type0) {|bytes_like bytes|}: parseable_serializeable bytes (group_info_tbs_nt bytes) = mk_parseable_serializeable ps_group_info_tbs_nt
 
+/// struct {
+///     GroupContext group_context;
+///     Extension extensions<V>;
+///     MAC confirmation_tag;
+///     uint32 signer;
+///     /* SignWithLabel(., "GroupInfoTBS", GroupInfoTBS) */
+///     opaque signature<V>;
+/// } GroupInfo;
+
 type group_info_nt (bytes:Type0) {|bytes_like bytes|} = {
   tbs: group_info_tbs_nt bytes;
   signature: mls_bytes bytes;
@@ -356,11 +627,21 @@ type group_info_nt (bytes:Type0) {|bytes_like bytes|} = {
 
 instance parseable_serializeable_group_info_nt (bytes:Type0) {|bytes_like bytes|}: parseable_serializeable bytes (group_info_nt bytes) = mk_parseable_serializeable ps_group_info_nt
 
+/// struct {
+///   opaque path_secret<V>;
+/// } PathSecret;
+
 type path_secret_nt (bytes:Type0) {|bytes_like bytes|} = {
   path_secret: mls_bytes bytes;
 }
 
 %splice [ps_path_secret_nt] (gen_parser (`path_secret_nt))
+
+/// struct {
+///   opaque joiner_secret<V>;
+///   optional<PathSecret> path_secret;
+///   PreSharedKeyID psks<V>;
+/// } GroupSecrets;
 
 type group_secrets_nt (bytes:Type0) {|bytes_like bytes|} = {
   joiner_secret: mls_bytes bytes;
@@ -373,12 +654,23 @@ type group_secrets_nt (bytes:Type0) {|bytes_like bytes|} = {
 
 instance parseable_serializeable_group_secrets_nt (bytes:Type0) {|bytes_like bytes|}: parseable_serializeable bytes (group_secrets_nt bytes) = mk_parseable_serializeable ps_group_secrets_nt
 
+/// struct {
+///   KeyPackageRef new_member;
+///   HPKECiphertext encrypted_group_secrets;
+/// } EncryptedGroupSecrets;
+
 type encrypted_group_secrets_nt (bytes:Type0) {|bytes_like bytes|} = {
   new_member: key_package_ref_nt bytes;
   encrypted_group_secrets: hpke_ciphertext_nt bytes;
 }
 
 %splice [ps_encrypted_group_secrets_nt] (gen_parser (`encrypted_group_secrets_nt))
+
+/// struct {
+///   CipherSuite cipher_suite;
+///   EncryptedGroupSecrets secrets<V>;
+///   opaque encrypted_group_info<V>;
+/// } Welcome;
 
 type welcome_nt (bytes:Type0) {|bytes_like bytes|} = {
   cipher_suite: cipher_suite_nt;
@@ -387,6 +679,23 @@ type welcome_nt (bytes:Type0) {|bytes_like bytes|} = {
 }
 
 %splice [ps_welcome_nt] (gen_parser (`welcome_nt))
+
+/// struct {
+///     ProtocolVersion version = mls10;
+///     WireFormat wire_format;
+///     select (MLSMessage.wire_format) {
+///         case mls_public_message:
+///             PublicMessage public_message;
+///         case mls_private_message:
+///             PrivateMessage private_message;
+///         case mls_welcome:
+///             Welcome welcome;
+///         case mls_group_info:
+///             GroupInfo group_info;
+///         case mls_key_package:
+///             KeyPackage key_package;
+///     };
+/// } MLSMessage;
 
 type mls_10_message_nt (bytes:Type0) {|bytes_like bytes|} =
   | [@@@ with_tag WF_mls_public_message] M_public_message: public_message_nt bytes -> mls_10_message_nt bytes
