fstar/treesync/code/MLS.TreeSync.TreeHash.fst
@@ -10,6 +10,11 @@ open MLS.Result
 
 #set-options "--fuel 1 --ifuel 1"
 
+/// struct {
+///     uint32 leaf_index;
+///     optional<LeafNode> leaf_node;
+/// } LeafNodeHashInput;
+
 type leaf_node_tree_hash_input_nt (bytes:Type0) {|bytes_like bytes|} (tkt:treekem_types bytes) = {
   leaf_index: nat_lbytes 4;
   [@@@ with_parser #bytes (ps_option (ps_leaf_node_nt tkt))]
@@ -19,6 +24,12 @@ type leaf_node_tree_hash_input_nt (bytes:Type0) {|bytes_like bytes|} (tkt:treeke
 %splice [ps_leaf_node_tree_hash_input_nt] (gen_parser (`leaf_node_tree_hash_input_nt))
 %splice [ps_leaf_node_tree_hash_input_nt_length] (gen_length_lemma (`leaf_node_tree_hash_input_nt))
 %splice [ps_leaf_node_tree_hash_input_nt_is_well_formed] (gen_is_well_formed_lemma (`leaf_node_tree_hash_input_nt))
+
+/// struct {
+///     optional<ParentNode> parent_node;
+///     opaque left_hash<V>;
+///     opaque right_hash<V>;
+/// } ParentNodeHashInput;
 
 type parent_node_tree_hash_input_nt (bytes:Type0) {|bytes_like bytes|} (tkt:treekem_types bytes) = {
   [@@@ with_parser #bytes (ps_option (ps_parent_node_nt tkt))]
@@ -30,6 +41,14 @@ type parent_node_tree_hash_input_nt (bytes:Type0) {|bytes_like bytes|} (tkt:tree
 %splice [ps_parent_node_tree_hash_input_nt] (gen_parser (`parent_node_tree_hash_input_nt))
 %splice [ps_parent_node_tree_hash_input_nt_length] (gen_length_lemma (`parent_node_tree_hash_input_nt))
 %splice [ps_parent_node_tree_hash_input_nt_is_well_formed] (gen_is_well_formed_lemma (`parent_node_tree_hash_input_nt))
+
+/// struct {
+///   NodeType node_type;
+///   select (TreeHashInput.node_type) {
+///     case leaf:   LeafNodeHashInput leaf_node;
+///     case parent: ParentNodeHashInput parent_node;
+///   };
+/// } TreeHashInput;
 
 type tree_hash_input_nt (bytes:Type0) {|bytes_like bytes|} (tkt:treekem_types bytes) =
   | [@@@ with_tag NT_leaf] LeafTreeHashInput: leaf_node: leaf_node_tree_hash_input_nt bytes tkt -> tree_hash_input_nt bytes tkt
