fstar/treekem/MLS.TreeKEM.NetworkTypes.fst
@@ -12,6 +12,11 @@ let tkt #bytes #bl = {
   ps_node_content = ps_hpke_public_key_nt;
 }
 
+/// struct {
+///     opaque kem_output<V>;
+///     opaque ciphertext<V>;
+/// } HPKECiphertext;
+
 type hpke_ciphertext_nt (bytes:Type0) {|bytes_like bytes|} = {
   kem_output: mls_bytes bytes;
   ciphertext: mls_bytes bytes;
@@ -19,12 +24,22 @@ type hpke_ciphertext_nt (bytes:Type0) {|bytes_like bytes|} = {
 
 %splice [ps_hpke_ciphertext_nt] (gen_parser (`hpke_ciphertext_nt))
 
+/// struct {
+///     HPKEPublicKey encryption_key;
+///     HPKECiphertext encrypted_path_secret<V>;
+/// } UpdatePathNode;
+
 type update_path_node_nt (bytes:Type0) {|bytes_like bytes|} = {
   encryption_key: hpke_public_key_nt bytes;
   encrypted_path_secret: mls_list bytes ps_hpke_ciphertext_nt;
 }
 
 %splice [ps_update_path_node_nt] (gen_parser (`update_path_node_nt))
+
+/// struct {
+///     LeafNode leaf_node;
+///     UpdatePathNode nodes<V>;
+/// } UpdatePath;
 
 type update_path_nt (bytes:Type0) {|bytes_like bytes|} = {
   leaf_node: leaf_node_nt bytes tkt;
